---
tags: 離散數學
aliase: 
created: 2023-02-08 15:19
modified: 星期三 8日 二月 2023 15:19:58
---

>2B~3C
# 03 mathematical induction
***
## Principle of mathematical indection:

suppose that S(n) is a statement involving the variable n with following properties:
(I)S(1) is true;
(II) if S(K) is true, then S(K+1) is true, for every k∈N
then S(n) is true for all n∈N

>induction basis = (I) check initial condition
>induction step = (II) induction hypothesis

***
### Example
Q1: show thar for all n∈N $\sum_{i=1}^{n}$(4i+3) = 2n<sup>2</sup> + 5n

<u>Proof</u>: 
<mark style="background: #FFB86CA6;">Induction basis</mark>: 
when n = 1 $\sum_{i=1}^{1}$(4i+3) = 7 = 2 x 1<sup>2</sup> + 5 x 1
<mark style="background: #FFB86CA6;">induction step</mark>: 
Assume that $\sum_{i=1}^{k}$(4i+3) = 2k<sup>2</sup> + 5k

Then $\sum_{i=1}^{k+1}$(4i+3) = $\sum_{i=1}^{k}$(4i+3) + 4(k+1) + 3
= 2k<sup>2</sup> + 5k + 4k + 7 
= 2k<sup>2</sup> + 9k + 7
= 2(k<sup>2</sup> + 2k + 1) + 5k + 5
= 2 x (k+1)<sup>2</sup> + 5 x (k+1)

By mathematical induction, this holds for all n∈N
***
### Example
Q2: show that for all n∈N $\sum_{i=1}^{n}$ i<sup>3</sup> = ($\frac{n(n+1))}{2}$)<sup>2</sup> 

<u>Proof</u>:
when n = 1 $\sum_{i=1}^{1}$ i<sup>3</sup> = 1 = ($\frac{2}{2}$)<sup>2</sup>
assume that $\sum_{i=1}^{k}$ i<sup>3</sup> = ($\frac{k(k+1))}{2}$)<sup>2</sup>   

$\sum_{i=1}^{k+1}$ i<sup>3</sup> = $\sum_{i=1}^{k}$ + (k+1)<sup>3</sup>
= ($\frac{k(k+1))}{2}$)<sup>2</sup> + (k+1)<sup>3</sup>
= (k+1)<sup>2</sup> ($\frac{k^2}{4}$ + k+1)
= (k+1)<sup>2</sup> $\frac{1}{4}$(k<sup>2</sup> + 4k+4)
= ($\frac{(k+1)(k+2))}{2}$)<sup>2</sup>
By mathematical induction, $\sum_{i=1}^{n}$ i<sup>3</sup> = ($\frac{n(n+1))}{2}$)<sup>2</sup>  for all n∈N

#### 在不知道答案時的算法 
使用 homogeneous recurrence of relation 齊次遞推
<u>ex</u>:
Let a<sub>n</sub> = $\sum_{i=1}^{n}$ i<sup>3</sup>  Then   a<sub>n</sub>-a<sub>n-1</sub>=n<sup>3</sup>   with a<sub>1</sub>=1   for n≥2



***
## Principle of mathematical induction - Alternative form

(I) S(n<sub>0</sub>), S(n<sub>0</sub>+1), ... , S(n<sub>1</sub>) are true;
>`initial condition 不見得只有一個，不一定從1開始，`

(II) if S(n<sub>0</sub>), S(n<sub>0</sub>+1), ... , S(K) are true for k≥n<sub>1</sub>;
> then S(k+1) is also true.

Then S(n) is true for all n≥N

### Example
Q: show that if a<sub>n</sub> is defined by a<sub>1</sub>=1,a<sub>2</sub>=5,
and a<sub>n+1</sub>= 5a<sub>n</sub> - 6a<sub>n-1</sub> for n≥2
then a<sub>n</sub> = 3<sup>n</sup> - 2<sup>n</sup> for all n∈N.
>要先確定 well define: 好的定義

- 使用數學歸納法 -> 知道答案的時候

Proof
<mark style="background: #FFB86CA6;">Induction basis</mark>: 
For n=1, 3<sup>1</sup> - 2<sup>1</sup> = 1 = a<sub>1</sub>
For n=2, 3<sup>2</sup> - 2<sup>2</sup> = 5 = a<sub>2</sub>

<mark style="background: #FFB86CA6;">Induction step</mark>:
Assume that the formula is true for both a<sub>k</sub> and a<sub>k-1</sub>
then a<sub>k+1</sub> = 5a<sub>k</sub> - 6a<sub>k-1</sub>
= 5(3<sup>k</sup>-2<sup>k</sup>) - 6(3<sup>k-1</sup>-2<sup>k-1</sup>)
= 5(3<sup>k</sup>-2<sup>k</sup>) - 2x3<sup>k</sup> - 3x2<sup>k</sup>
= 3x3<sup>k</sup> - 2x2<sup>k</sup>
= (3<sup>k+1</sup>-2<sup>k+1</sup>)

Therefore, by mathematical induction, a<sub>n</sub>=3<sup>n</sup>-2<sup>n</sup> for all n∈N
***
## Everybody is rich？

Theorm: Everybody is rich
<u>consider</u> S(n) given any collection of n persons, if at least one of them is rich, they are all rich

<mark style="background: #FFB86CA6;">Induction basis</mark>:
S(1): 只有一人 -> 必須有錢

<mark style="background: #FFB86CA6;">Induction step</mark>:
Assume S(K)成立 -> 
Consider K+1 persons {a<sub>1</sub>, a<sub>2</sub>, a<sub>3</sub> ... a<sub>k</sub>, a<sub>k+1</sub>}
>此時只須證明 a<sub>k+1</sub>這人有錢，那所有人都有錢

Suppose a<sub>1</sub> is rich
then {a<sub>1</sub>, a<sub>2</sub>, a<sub>3</sub> ... a<sub>k</sub>} is a set of k persons, since a<sub>1</sub> is rich by S(K).
-> a<sub>1</sub>, a<sub>2</sub>, a<sub>3</sub> ... a<sub>k</sub> are all rich

Also consider {a<sub>1</sub>, a<sub>2</sub>, a<sub>3</sub> ... a<sub>k-1</sub>, a<sub>k+1</sub>}有K個人, since a<sub>1</sub> is rich by S(K).
>去除a<sub>k</sub> {a<sub>1</sub>, a<sub>2</sub>, a<sub>3</sub> ... a<sub>k-1</sub>, a<sub>k+1</sub>}性質成立 -> a<sub>k+1</sub>有錢

a<sub>1</sub>, a<sub>2</sub>, a<sub>3</sub> ... a<sub>k-1</sub>, a<sub>k+1</sub> are all rich
k個人只要有一人有錢，那所有人都有錢
根據S(K)性質可推得a<sub>k+1</sub>有錢，這符合命題

by mathematical, S(n) is true for all n∈N

<mark style="background: #FFB8EBA6;">反證法</mark>:
設第k+1人沒錢，但根據S(K)性質我們可以知道 -> 前K人是有錢
但根據命題敘述只要有一人有錢所有人都有錢 -> 與第K+1人沒錢衝突了
衝突 -> 命題不正確 -> S(K)=false -> 與我們的假設S(K)=true衝突

所以，第k+1人必須有錢，不然會與S(K)衝突
***

>[!error]+
>上面的推論都是錯的，當k=1時無法帶入，因為a<sub>1</sub>被固定了