---
tags: 離散數學
aliase: 
created: 2023-02-18 19:40
modified: 星期六 18日 二月 2023 19:40:01
---

>3C~4B
# 04 函數
***
Let A and B be nonempty sets. 
<u>Def</u> A function f: A→B is a rule that assigns to each element a∈A a unique element b∈B
>→不是implies，是對應的意思

>[!col]+
>![[function_graph]]
>>[!col]+
>A: domain of f
>B: codomain of f
>f(a) = b
>f(A)={f(a):a∈A} range of A
>f(A) is subset of B

## Type
### injective function
<u>Def</u> A function f: A→B is called <u>one-to-one</u> or <u>injective</u>, if f(a<sub>1</sub>)=f(a<sub>2</sub>) implies a<sub>1</sub>=a<sub>2</sub> ( or equivalently, a<sub>1</sub>≠a<sub>2</sub> implies f(a<sub>1</sub>)≠f(a<sub>2</sub>) )
>"f: A→B": injective 嵌射、單射
>"f" is called injection or injective function or one-to-one function

- |B|≥|A|
- 不存在一對多、多對一
- <mark style="background: #FFB86CA6;">一對一</mark> 映射到不同的b
### Sujective function
<u>Def</u> function f:A→B is called <u>onto</u> or <u>surjective</u>. if f(A)=B, i.e, for all b∈B there is at least one a∈A with f(a)=b. And f is called <u>sujection</u>.

>"f: A→B": sujective 蓋射
>"f" is called sujection or sujective function
- |A|≥|B|
- 不存在一對多
- <mark style="background: #FFB86CA6;">f(A) = B</mark> b所有元素需被映射
### bijective function
<u>Def</u> function f:A→B is called <u>one-to-one correspond</u> or <u>bijective</u> (a <u>bijection</u>) if f is both one to one and onto ( or equivalently, both injective and sujective )

>"f: A→B": bijective 對射
>"f" is called bijection or bijective function
- |A|=|B|
- injetive sujective <mark style="background: #FFB86CA6;">同時成立</mark>

***
## Compositive function
<u>Def</u> The compositr function of f:A→B and g:B→C, denoted g∘f:A→C, is defined by (g∘f)(a) = g(f(a)), a∈A 

<u>Remark</u> if f:A→B, g:B→C, and h:C→D, (h∘g)∘f = h∘(g∘f)

<u>Property</u> f:A→B and g:B→C
1. if f and g are injective, then so is g∘f
2. if f and g are sujective, then so is g∘f
3. if f and g are bijective, then so is g∘f

<mark style="background: #FFB86CA6;">Proof</mark>:
1. Suppose (g∘f)(a<sub>1</sub>) = (g∘f)(a<sub>2</sub>)
⇒ g(f(a<sub>1</sub>)) = g(f(a<sub>2</sub>)) 
⇒ f(a<sub>1</sub>) = f(a<sub>2</sub>) `'Since g is injective'`
⇒ a<sub>1</sub> = a<sub>2</sub> `'Since f is injective'`
<mark style="background: #FF5582A6;">∴</mark> g∘f is injective

2. If g is sujective
then for all c∈C there exist some b∈B with g(b)=c and if f is sujective, there exist some a∈A with f(a)=b, Thus c=g(b) = g(f(a)) = (g∘f)(a)
<mark style="background: #FF5582A6;">∴</mark> g∘f is injective

3. The proof follows directly from 1. and 2.
***
### inverse
<u>Def</u>: A funciton f:A→B is said to be <u>invertible</u> if there is a function g:B→A, such that (g∘f)(a)=a a∈A, (f∘g)(b)=b b∈B

- 如果只有一個成立通常稱為左/右inverse 
- inverse必須 left/right都成立

<u>Remark</u>: g is called <u>an inverse of</u> f

<u>Property</u>: if f has an inverse, then it is unique

<mark style="background: #FFB86CA6;">Proof</mark>: Suppose g and g' both satisfy the condition for an inverse of f:A→B, i.e (g∘f)(a)=a, (f∘g)(b)=b
(g'∘f)(a)=a, (f∘g')(b)=b For all b∈B.
g(b)
= (g'∘f)(g(b))
= g'(f(g(b)))
= g'((f∘g)(b))
= g'(b)
<mark style="background: #FF5582A6;">∴</mark> g = g'

Notation: Inverse of f: f<sup>-1</sup>
Note that (f<sup>-1</sup>)<sup>-1</sup> = f

<u>Property</u>: A function is invetible iff it is bijective

<mark style="background: #FFB86CA6;">Proof</mark>: "left" 
Suppose f:A→B is bijective For all b∈B, there exists a <u>unique</u> a∈A such that f(a) = b. The rule g(b)=a define a function from B to A.
Then (g∘f)(a) = g(f(a)) = f(b) = a and (f∘g)(b) = f(g(b)) = f(a) = b.
Hence g is an inverse of f and f is invertible.

<mark style="background: #FFB86CA6;">Proof</mark>: "right" 
Suppose f is invertible and has inverse f<sup>-1</sup>.
For all b∈B, we know that f(f<sup>-1</sup>(b))=b
So letting a = f<sup>-1</sup>(b)∈A yields f(a) = b.
Thus f is sujective
Now suppose f(a<sub>1</sub>)=f(a<sub>2</sub>), for a<sub>1</sub>, a<sub>2</sub>∈A
⇒ f<sup>-1</sup>(f(a<sub>1</sub>)) = f<sup>-1</sup>(f(a<sub>2</sub>)) 
⇒ a<sub>1</sub> = a<sub>2</sub>
Hence f is injective, therefore f is bijective.
***
## Example
<u>Q</u>: A={1, 2, 3} B={x, y}
How many functions f:A→B are injective, sujective or bijective ?

There are totally 2x2x2=8 different functions
f:A→B

>[!col]+
>| a         | f1 | f2 | f3 | f4 | f5 | f6 | f7 | f8 |
>|:----------|:---|:---|:---|:---|:---|:---|:---|:---|
>|         1 | x  | x  | x  | x  | y  | y  | y  | y  |
>|         2 | x  | x  | y  | y  | x  | x  | y  | y  |
>|         3 | x  | y  | x  | y  | x  | y  | x  | y  |
>|           |    |    |    |    |    |    |    |    |
>| injective | N  | N  | N  | N  | N  | N  | N  | N  |
>| sujective | N  | Y  | Y  | Y  | Y  | Y  | Y  | N  |
>| bijective | N  | N  | N  | N  | N  | N  | N  | N  |  
>>[!col]+
>Ans: 
>injective:0
>sujective:6
>bijective:0

<mark style="background: #FFB86CA6;">其他算法</mark>
<u>總函數量</u>: |B|<sup>|A|</sup>
>2<sup>3</sup>=8

<u>injective</u>:
比較基數: |A|≤|B|

P$_{|A|}^{|B|}$ = Ans

<mark style="background: #FF5582A6;">sujective</mark>: 
>$(_{2}^{3})+(_{1}^{3})=6$
>$8-2=6$

<u>bijective</u>:
比較基數: |A|=|B|
P$_{|A|}^{|B|}$ = Ans






